state/CooperativeMultiThreadingWithIndexTShareableTyp.fst
@@ -180,7 +180,7 @@ let rec scheduler (fuel:nat) (#t:full_ground_typ) (r : ref (to_Type t)) (tasks:l
 =
   witness (contains_pred r);
   witness (is_shareable r);
-  let counter_st = sst_read counter in
+  let counter_st = lr_read counter in
   let hist = counter_st._1 in
   let i = counter_st._2 in
   let inactive = counter_st._3 in
@@ -196,7 +196,7 @@ let rec scheduler (fuel:nat) (#t:full_ground_typ) (r : ref (to_Type t)) (tasks:l
     lemma_fairness_step (length tasks) hist i;
     lemma_prefix_of_append hist [i];
     let counter_st' : counter_state (length tasks) = (| hist @ [i], (incr #(length tasks') i), inactive' |) in
-    let () = sst_write counter counter_st' in
+    let () = lr_write counter counter_st' in
     scheduler (fuel-1) r tasks' counter
   | Yield k' ->
     let inactive' = 0 in
@@ -205,7 +205,7 @@ let rec scheduler (fuel:nat) (#t:full_ground_typ) (r : ref (to_Type t)) (tasks:l
     lemma_fairness_step (length tasks) hist i;
     lemma_prefix_of_append hist [i];
     let counter_st' : counter_state (length tasks) = (| hist @ [i], (incr #(length tasks') i), inactive' |) in
-    let () = sst_write counter counter_st' in
+    let () = lr_write counter counter_st' in
     scheduler (fuel-1) r tasks' counter
   end
 #pop-options
@@ -218,27 +218,27 @@ let run (fuel : nat) (#t:full_ground_typ) (init:to_Type t) (tasks:list (r:ref (t
       forall_refs_heap contains_pred h0 init /\ 
       forall_refs_heap is_shareable h0 init)) 
     (ensures (fun h0 _ h1 -> True)) =
-  let counter = sst_alloc #_ #(counter_preorder _) (counter_init (length tasks)) in
-  let s : ref (to_Type t) = sst_alloc_shared init in
+  let counter = lr_alloc #_ #(counter_preorder _) (counter_init (length tasks)) in
+  let s : ref (to_Type t) = lr_alloc_shared init in
   let tasks = map (fun (f : (r:ref (to_Type t)) -> continuation r unit) -> f s) tasks in
   scheduler fuel s tasks counter;
-  sst_read s
+  lr_read s
   
 let res_a (r : ref int) : continuation r unit = fun () ->
   recall (contains_pred r);
   recall (is_shareable r);
-  let () = sst_write_ref r 42 in
+  let () = lr_write_ref r 42 in
   Return ()
 
 let res_b (r : ref int) : continuation r unit = fun () ->
   recall (contains_pred r);
   recall (is_shareable r);
-  let j = sst_read r in
-  let m = sst_alloc #int #(FStar.Heap.trivial_preorder _) 42 in
+  let j = lr_read r in
+  let m = lr_alloc #int #(FStar.Heap.trivial_preorder _) 42 in
   Yield (fun () ->
     recall (contains_pred r);
     recall (is_shareable r);
-    let () = sst_write r j in
+    let () = lr_write r j in
     Return ())
 
 let nmm () : LR int (requires (fun _ -> True)) (ensures (fun _ _ _ -> True)) = run 5000 0 [res_a; res_b]
