state/Examples.Guess.fst
@@ -25,12 +25,12 @@ type play_guess_type a3p =
 val play_guess : play_guess_type c3p
 let play_guess args =
   let player, (pick, (l, r)) = args in
-  let counter : mref int (fun v' v'' -> b2t (v' <= v'')) = sst_alloc 0 in
+  let counter : mref int (fun v' v'' -> b2t (v' <= v'')) = lr_alloc 0 in
   sst_encapsulate counter;
   witness (contains_pred counter);witness (is_encapsulated counter);
   let cb (g:int) : LR cmp (fun _ -> True) (fun h0 r h1 -> h0 `hrel_c` h1) = (
     recall (contains_pred counter);recall (is_encapsulated counter);
-    sst_write counter ((sst_read counter) + 1);
+    lr_write counter ((lr_read counter) + 1);
     if g = pick then EQ else if pick < g then LT else GT) in
   let final_guess = player ((l,r),cb) in
   if pick = final_guess then (Inl (true, !counter))
