state/Examples.Hello.fst
@@ -12,20 +12,20 @@ let hello0 ()
   : LR (ref int)
     (requires (fun h0 -> True))
     (ensures (fun h0 _ h1 -> True)) =
-    sst_alloc_shareable #SNat 1
+    lr_alloc_shareable #SNat 1
 
 let hello ()
   : LR unit
     (requires (fun h0 -> True))
     (ensures (fun h0 () h1 -> True)) =
-    let ref_ll = sst_alloc_shareable #SNat 1 in 
+    let ref_ll = lr_alloc_shareable #SNat 1 in 
     ()
 
 let hello_read_write ()
   : LR unit
     (requires (fun h0 -> False))
     (ensures (fun h0 () h1 -> True)) =
-    let ref = sst_alloc_shareable #SNat 1 in 
+    let ref = lr_alloc_shareable #SNat 1 in 
     let v = !ref in
     ref := v + 1;
     ()
